@prefix rdf: <http://www.w3.org/1999/02/22-rdf-syntax-ns#>.
@prefix rdfs: <http://www.w3.org/2000/01/rdf-schema#>.
@prefix owl: <http://www.w3.org/2002/07/owl#>.
@prefix xsd: <http://www.w3.org/2001/XMLSchema#>.
@prefix dce: <http://purl.org/dc/elements/1.1/>.
@prefix skos: <http://www.w3.org/2004/02/skos/core#>.
@prefix irw: <http://www.ontologydesignpatterns.org/ont/web/irw.owl#>.
@prefix foaf: <http://xmlns.com/foaf/0.1/>.
@prefix event: <http://eulersharp.sourceforge.net/2003/03swap/event#>.
@prefix doc: <http://eulersharp.sourceforge.net/2003/03swap/document#>.
@prefix coding: <http://eulersharp.sourceforge.net/2003/03swap/coding#>.

<http://eulersharp.sourceforge.net/2003/03swap/coding>
        a owl:Ontology;
        dce:creator """Hans Cools, MD; Agfa Healthcare/Belgium"""@en;
        dce:publisher """Agfa Healthcare/Belgium"""@en;
        dce:description """Formal general description of coding."""@en;
        dce:format """OWL Full"""@en;
        rdfs:seeAlso <http://www.w3.org/2004/02/skos/core>, <http://www.agfa.com/w3c/2009/clinicalSKOSSchemes>.

#
# CLASSES
#

coding:Code
        a rdfs:Class;
        rdfs:isDefinedBy <http://eulersharp.sourceforge.net/2003/03swap/coding#>;
        rdfs:label """code"""@en;
        skos:definition """Applied or converted form of information wherein one thing is replaced by another thing."""@en;
        rdfs:comment """A code system is declared using <http://www.w3.org/2004/02/skos/core#inScheme>. A system version is declared using <http://purl.org/dc/terms/hasVersion>."""@en;
        rdfs:subClassOf doc:Content.

#
# PROPERTIES
#

coding:hasCode
        a owl:ObjectProperty, owl:InverseFunctionalProperty;
        rdfs:isDefinedBy <http://eulersharp.sourceforge.net/2003/03swap/coding#>;
        skos:definition """Specifying a code for something."""@en;
        rdfs:subPropertyOf event:objectOf;
        rdfs:domain rdfs:Resource;
        rdfs:range coding:Code.

coding:codes
        a owl:ObjectProperty, owl:FunctionalProperty;
        rdfs:isDefinedBy <http://eulersharp.sourceforge.net/2003/03swap/coding#>;
        skos:definition """Specifying something that has a code."""@en;
        rdfs:subPropertyOf doc:about;
        owl:inverseOf coding:hasCode;
        rdfs:domain coding:Code;
        rdfs:range rdfs:Resource.

coding:hasCodeValue
        a owl:DatatypeProperty, owl:InverseFunctionalProperty, owl:FunctionalProperty;
        rdfs:isDefinedBy <http://eulersharp.sourceforge.net/2003/03swap/coding#>;
        skos:definition """Specifying a code value."""@en;
        rdfs:domain coding:Code;
        rdfs:range rdfs:Datatype.

coding:hasCodeAuthority
        a rdf:Property;
        rdfs:isDefinedBy <http://eulersharp.sourceforge.net/2003/03swap/coding#>;
        skos:definition """Specifying an organization governing the code system, e.g. a government for a social security number."""@en;
        rdfs:domain coding:Code;
        rdfs:range foaf:Organization.

coding:hasCodeExpirationDate
        a owl:DatatypeProperty, owl:FunctionalProperty;
        rdfs:isDefinedBy <http://eulersharp.sourceforge.net/2003/03swap/coding#>;
        skos:definition """Specifying the date on which a code stops to be valid."""@en;
        rdfs:subPropertyOf event:expires;
        rdfs:domain coding:Code;
        rdfs:range xsd:dateTime.

coding:hasMappingCode
        a owl:DatatypeProperty;
        rdfs:isDefinedBy <http://eulersharp.sourceforge.net/2003/03swap/coding#>;
        skos:definition """Specifying for something a code of a SKOS concept matching a class that something is an instance of."""@en;
        owl:propertyChainAxiom (rdf:type skos:mappingRelation skos:notation);
        rdfs:domain rdfs:Resource;
        rdfs:range rdfs:Datatype.

coding:hasExactCode
        a owl:DatatypeProperty;
        rdfs:isDefinedBy <http://eulersharp.sourceforge.net/2003/03swap/coding#>;
        skos:definition """Specifying for something a code of a SKOS concept matching exactly a class the instance is member of."""@en;
        rdfs:subPropertyOf coding:hasMappingCode;
        owl:propertyChainAxiom (rdf:type skos:exactMatch skos:notation);
        rdfs:domain rdfs:Resource;
        rdfs:range rdfs:Datatype.

coding:hasBroadCode
        a owl:DatatypeProperty;
        rdfs:isDefinedBy <http://eulersharp.sourceforge.net/2003/03swap/coding#>;
        skos:definition """Specifying for something a code of a SKOS concept being broader than a class the instance is member of."""@en;
        rdfs:subPropertyOf coding:hasMappingCode;
        owl:propertyChainAxiom (rdf:type skos:broadMatch skos:notation);
        rdfs:domain rdfs:Resource;
        rdfs:range rdfs:Datatype.

coding:hasNarrowCode
        a owl:DatatypeProperty;
        rdfs:isDefinedBy <http://eulersharp.sourceforge.net/2003/03swap/coding#>;
        skos:definition """Specifying for something a code of a SKOS concept being narrower than a class the instance is member of."""@en;
        rdfs:subPropertyOf coding:hasMappingCode;
        owl:propertyChainAxiom (rdf:type skos:narrowMatch skos:notation);
        rdfs:domain rdfs:Resource;
        rdfs:range rdfs:Datatype.

