@prefix dce: <http://purl.org/dc/elements/1.1/>.
@prefix owl:  <http://www.w3.org/2002/07/owl#>.
@prefix rdfs: <http://www.w3.org/2000/01/rdf-schema#>.
@prefix xsd: <http://www.w3.org/2001/XMLSchema#>.
@prefix skos: <http://www.w3.org/2004/02/skos/core#>.
@prefix digproc: <http://eulersharp.sourceforge.net/2003/03swap/digitalProcedure#>.
@prefix event: <http://eulersharp.sourceforge.net/2003/03swap/event#>.
@prefix sparql: <http://eulersharp.sourceforge.net/2003/03swap/sparql#>.
@prefix sparante: <http://eulersharp.sourceforge.net/2003/03swap/sparqlAnalysisTemplate#>.
@prefix sparan: <http://eulersharp.sourceforge.net/2003/03swap/sparqlAnalysis#>.

<http://eulersharp.sourceforge.net/2003/03swap/sparqlAnalysis#>
        a owl:Ontology;
        dce:title """SPARQL Analysis"""@en;
        dce:creator """Hans Cools, MD; Agfa Healthcare, Belgium"""@en;
        dce:contributor """Kristof Depraetere, Boris De Vloed, Giovanni Mels, ir; Agfa Healthcare, Belgium"""@en;
        dce:publisher """Agfa Healthcare, Belgium"""@en;
        dce:description """Formal description of RDF data analysis using SPARQL."""@en;
        dce:format """OWL Full"""@en.

#
# CLASSES
#

sparan:AnalysisQuery
        a rdfs:Class;
        rdfs:isDefinedBy <http://eulersharp.sourceforge.net/2003/03swap/sparqlAnalysis#>;
        rdfs:label """analysis SPARQL query"""@en;
        skos:definition """SPARQL query formulating what RDF data has to be analysed."""@en.
        #rdfs:subClassOf sparql:Query.

sparan:ClinicalAnalysisQuery
        a rdfs:Class;
        rdfs:isDefinedBy <http://eulersharp.sourceforge.net/2003/03swap/sparqlAnalysis#>;
        rdfs:label """clinical analysis SPARQL query"""@en;
        skos:definition """SPARQL query formulating what clinical RDF data has to be analysed."""@en;
        rdfs:subClassOf sparan:AnalysisQuery, [
                a owl:Restriction; owl:onProperty sparql:hasTemplate; owl:someValuesFrom sparante:ClinicalAnalysisQueryTemplate], [
                a owl:Restriction; owl:onProperty sparql:hasBinding; owl:someValuesFrom sparante:ClinicalAnalysisQueryTemplateBinding], [
                a owl:Restriction; owl:onProperty sparan:hasDataSetQuery; owl:someValuesFrom sparan:ClinicalDataSetQuery], [
                a owl:Restriction; owl:onProperty digproc:hasResult; owl:someValuesFrom sparan:ClinicalAnalysisResult].

sparan:SubmittedClinicalAnalysisQuery
        a rdfs:Class;
        rdfs:isDefinedBy <http://eulersharp.sourceforge.net/2003/03swap/sparqlAnalysis#>;
        rdfs:label """submitted clinical analysis SPARQL query"""@en;
        skos:definition """SPARQL query, formulating what clinical RDF data has to be analysed, in the submitted state."""@en;
        rdfs:subClassOf sparan:ClinicalAnalysisQuery.

sparan:CancelledClinicalAnalysisQuery
        a rdfs:Class;
        rdfs:isDefinedBy <http://eulersharp.sourceforge.net/2003/03swap/sparqlAnalysis#>;
        rdfs:label """cancelled clinical analysis SPARQL query"""@en;
        skos:definition """SPARQL query, formulating what clinical RDF data has to be analysed, in the unsubmitted state."""@en;
        rdfs:subClassOf sparan:ClinicalAnalysisQuery.

sparan:CompletedClinicalAnalysisQuery
        a rdfs:Class;
        rdfs:isDefinedBy <http://eulersharp.sourceforge.net/2003/03swap/sparqlAnalysis#>;
        rdfs:label """completed clinical analysis SPARQL query"""@en;
        skos:definition """SPARQL query, formulating what clinical RDF data has to be analysed, in the completed state."""@en;
        rdfs:subClassOf sparan:ClinicalAnalysisQuery.

sparan:DataSetQuery
        a rdfs:Class;
        rdfs:isDefinedBy <http://eulersharp.sourceforge.net/2003/03swap/sparqlAnalysis#>;
        rdfs:label """data set SPARQL query"""@en;
        skos:definition """SPARQL query on a repository with RDF data to be analysed."""@en.
#       rdfs:subClassOf sparql:Query.

sparan:ClinicalDataSetQuery
        a rdfs:Class;
        rdfs:isDefinedBy <http://eulersharp.sourceforge.net/2003/03swap/sparqlAnalysis#>;
        rdfs:label """clinical data set SPARQL query"""@en;
        skos:definition """SPARQL query on a repository with clinical RDF data to be analysed."""@en;
        rdfs:subClassOf sparan:DataSetQuery.

sparan:InvalidClinicalDataSetQuery
        a rdfs:Class;
        rdfs:isDefinedBy <http://eulersharp.sourceforge.net/2003/03swap/sparqlAnalysis#>;
        rdfs:label """invalid clinical data set SPARQL query"""@en;
        skos:definition """Invalidated SPARQL query on a repository with clinical RDF data to be analysed."""@en;
        rdfs:subClassOf sparan:ClinicalDataSetQuery.

sparan:ClinicalAnalysisResult   # result without completion = draft
        a rdfs:Class;
        rdfs:isDefinedBy <http://eulersharp.sourceforge.net/2003/03swap/sparqlAnalysis#>;
        rdfs:label """clinical analysis result"""@en;
        skos:definition """SPARQL result of analysis of clinical RDF data."""@en;
        rdfs:subClassOf [ # containing sparql:Result
                a owl:Restriction; owl:onProperty sparql:hasBinding; owl:someValuesFrom sparante:ClinicalAnalysisResultBinding].

sparan:InvalidClinicalAnalysisResult
        a rdfs:Class;
        rdfs:isDefinedBy <http://eulersharp.sourceforge.net/2003/03swap/sparqlAnalysis#>;
        rdfs:label """invalid clinical analysis result"""@en;
        skos:definition """Invalidated SPARQL result of analysis of clinical RDF data."""@en;
        rdfs:subClassOf sparan:ClinicalAnalysisResult.

sparan:DataRepository   # Digital repository, also known as a virtual or digital library
        a rdfs:Class.

sparan:ClinicalDataRepository
        a rdfs:Class;
        rdfs:subClassOf sparan:DataRepository.

#
# PROPERTIES
#

sparan:hasDataRepository
        a owl:ObjectProperty;
        rdfs:isDefinedBy <http://eulersharp.sourceforge.net/2003/03swap/sparqlAnalysis#>;
        skos:definition """Specifying a data repository to execute a data set SPARQL query on."""@en;
        rdfs:domain sparan:DataSetQuery;
        rdfs:range sparan:DataRepository.

sparan:dataRepositoryOf
        a owl:ObjectProperty;
        rdfs:isDefinedBy <http://eulersharp.sourceforge.net/2003/03swap/sparqlAnalysis#>;
        skos:definition """Specifying a data set SPARQL query to be executed on a data repository."""@en;
        owl:inverseOf sparan:hasDataRepository;
        rdfs:domain sparan:DataRepository;
        rdfs:range sparan:DataSetQuery.

sparan:hasDataSetQuery
        a owl:ObjectProperty;
        rdfs:isDefinedBy <http://eulersharp.sourceforge.net/2003/03swap/sparqlAnalysis#>;
        skos:definition """Specifying a data set SPARQL query of an analysis SPARQL query."""@en;
        rdfs:domain sparan:AnalysisQuery;
        rdfs:range sparan:DataSetQuery.

sparan:dataSetQueryOf
        a owl:ObjectProperty;
        rdfs:isDefinedBy <http://eulersharp.sourceforge.net/2003/03swap/sparqlAnalysis#>;
        skos:definition """Specifying an analysis SPARQL query of a data set SPARQL query."""@en;
        owl:inverseOf sparan:hasDataSetQuery;
        rdfs:domain sparan:DataSetQuery;
        rdfs:range sparan:AnalysisQuery.

