@prefix dce: <http://purl.org/dc/elements/1.1/>.
@prefix owl: <http://www.w3.org/2002/07/owl#>.
@prefix rdfs: <http://www.w3.org/2000/01/rdf-schema#>.
@prefix skos: <http://www.w3.org/2004/02/skos/core#>.
@prefix xsd: <http://www.w3.org/2001/XMLSchema#>.
@prefix event: <http://eulersharp.sourceforge.net/2003/03swap/event#>.
@prefix wesc: <http://eulersharp.sourceforge.net/2003/03swap/weekScheme#>.

<http://eulersharp.sourceforge.net/2003/03swap/weekScheme#>
        a owl:Ontology;
        dce:title """Week Scheme"""@en;
        dce:creator """Hans Cools, MD; Agfa Healthcare/Belgium"""@en;
        dce:contributor """Jos De Roo; Agfa Healthcare/Belgium"""@en;
        dce:publisher """Agfa Healthcare/Belgium"""@en;
        dce:description """Formal general description of a working week scheme."""@en;
        rdfs:comment """Used in e.g. rules to calculate availbility knowing opening hours."""@en;
        dce:format """OWL Full"""@en.

#
# CLASSES
#

# Among others, following classes are available in http://eulersharp.sourceforge.net/2003/03swap/event#.
# event:Availability
# event:Unavailability
# event:Day
# event:Weekday
# event:Month

wesc:Day
        a rdfs:Class;
        rdfs:isDefinedBy <http://eulersharp.sourceforge.net/2003/03swap/weekScheme#>;
        rdfs:label """working day"""@en;
        skos:definition """Event in which there is a day working scheme."""@en;
        rdfs:subClassOf event:Event.

wesc:Duty
        a rdfs:Class;
        rdfs:isDefinedBy <http://eulersharp.sourceforge.net/2003/03swap/weekScheme#>;
        rdfs:label """duty"""@en;
        skos:definition """Event in which there is a different working scheme from the day working scheme."""@en;
        rdfs:subClassOf event:Event.

#
# Properties
#

# Among others, following properties are available in http://eulersharp.sourceforge.net/2003/03swap/event#.
# event:hasPriority
# event:begins
# event:ends
# event:hasDuration
# event:hasSnapshot
# event:hasNow

#wesc:weekStart # currently not needed
#       skos:definition """Specifying the actual week start date and time."""@en;
#       a owl:DatatypeProperty, owl:FunctionalProperty;
#       rdfs:domain event:Event;
#       rdfs:range xsd:dateTime.

wesc:hasDayStart
        a owl:DatatypeProperty, owl:FunctionalProperty;
        skos:definition """Specifying the start of a day period relatively to the week start."""@en;
        rdfs:domain wesc:Day;
        rdfs:range xsd:duration.

wesc:hasDayEnd
        a owl:DatatypeProperty, owl:FunctionalProperty;
        skos:definition """Specifying the end of a day period relatively to the week start."""@en;
        rdfs:domain wesc:Day;
        rdfs:range xsd:duration.

wesc:hasDutyStart
        a owl:DatatypeProperty, owl:FunctionalProperty;
        skos:definition """Specifying the start of a duty period relatively to the week start."""@en;
        rdfs:domain wesc:Duty;
        rdfs:range xsd:duration.

wesc:hasDutyEnd
        a owl:DatatypeProperty, owl:FunctionalProperty;
        skos:definition """Specifying the end of a duty period relatively to the week start."""@en;
        rdfs:domain wesc:Duty;
        rdfs:range xsd:duration.


