@prefix : <http://eulergui.sf.net/ontology/project.owl.n3#>.
@prefix owl:  <http://www.w3.org/2002/07/owl#> .
@prefix rdfs: <http://www.w3.org/2000/01/rdf-schema#> .
@prefix rdf: <http://www.w3.org/1999/02/22-rdf-syntax-ns#> .
@prefix xsd:  <http://www.w3.org/2001/XMLSchema#> .

# The EulerGUI Project ontology $Id$

:URLSource a owl:Class
    ; rdfs:comment """just an auxiliary class for a data source that has
                      either a dereferenciable URL or a relative URL."""
 .

:RDFImport rdfs:subClassOf :URLSource
     ; a owl:Class
     ; rdfs:label "RDF Import"
     ; rdfs:comment """RDF import means that a non RDF source like plain XML, XMI, etc
                       is converted in a well defined way into an RDF/N3 document."""
 .

:hasRDFImport a owl:ObjectProperty
     ; rdfs:domain owl:Ontology
     ; rdfs:range :RDFImport
     ; rdfs:label "has RDF Import"
     ; rdfs:comment """In addition to its regular content, an owl:Ontology
                       has RDF Imports that aware applications add to the regular
                       content."""
.

:hasN3Source a owl:ObjectProperty
     ; rdfs:domain owl:Ontology
     ; rdfs:range :RDFImport
     ; rdfs:label "has RDF Import"
     ; rdfs:comment """In addition to its regular content, an owl:Ontology
                       has RDF Imports that aware applications add to the regular
                       content.""".

:hasURL a owl:DatatypeProperty
     ; rdfs:domain :URLSource
     ; rdfs:range xsd:anyURI
     ; rdfs:label "has an (absolute) URI"
     ; rdfs:comment "a dereferenciable URI for the RDF import"
 .
:hasRelativeURL a owl:DatatypeProperty
     ; rdfs:domain :URLSource
     ; rdfs:range xsd:string
     ; rdfs:label "has a relative URI"
     ; rdfs:comment """a relative URI for the RDF import, relative to the base URI of
                       the importing Ontology.
                       An RDFImport has either a relative URI, or an (absolute) URI,
                       but not both."""
 .

:isActivated a owl:DatatypeProperty
     ; rdfs:domain :RDFImport
     ; rdfs:range xsd:boolean
     ; rdfs:label "is this RDF source activated during inferencing?"
     ; rdfs:comment """It is convenient to have data sources belonging to
                       the project just as reference or trial."""
 .

:hasN3Query a owl:ObjectProperty
     ; rdfs:domain owl:Ontology
     ; rdfs:range :URLSource
     ; rdfs:label "has an (absolute) URI"
     ; rdfs:comment "a dereferenciable URI for the RDF import"
.

:hasFormat a owl:ObjectProperty
    ; rdfs:domain :URLSource
    ; rdfs:range  [
        owl:oneOf (
            <http://www.w3.org/1999/02/22-rdf-syntax-ns#> # RDF/XML (possibly OWL)
            <http://www.w3.org/TeamSubmission/turtle/> # Turtle (no formulas and rules)
            <http://www.w3.org/TeamSubmission/n3/> # N3 (possibly formulas and rules)
            <http://www.w3.org/TR/owl2-xml-serialization/> # OWL/XML
            # plain XML, non RDF/XML nor OWL/XML nor XMI
            <http://www.w3.org/XML/1998/namespace>
            <http://schema.omg.org/spec/XMI> # XMI (UML, eCore, MOF, etc)
        ) ]
    ; rdfs:comment """In most cases, by looking at the HTTP Content-type,
                      and/or the extension, or even the beginning of document,
                      the application is able to guess the file format,
                      so this property is facultative."""
 .

:isMainQuery
      a owl:DatatypeProperty ;
      rdfs:comment "???" ;
      rdfs:domain <http://my.com/_domain_> ;
      rdfs:label "isMainQuery" ;
      rdfs:range <http://my.com/_range_> .

:postProcessing
      a       rdf:Property ;
      rdfs:comment "???" ;
      rdfs:domain owl:Ontology ;
      rdfs:label "postProcessing" ;
      rdfs:range <http://my.com/_range_> .

:subproject
      a       rdf:Property ;
      rdfs:comment "???" ;
      rdfs:domain owl:Ontology ;
      rdfs:label "subproject" ;
      rdfs:range <http://my.com/_range_> .


